Add decomposition rule

examples/02-proof-rules/CompositionRules.v
@@ -2,24 +2,111 @@ Require Import tulip.tla.TLA.
 
 #[local] Open Scope tla_scope.
 
-Section rules.
+(* ========================================================================== *)
+(* The proof rules are from (unless otherwise stated):                        *)
+(* > Leslie Lamport. 2026. A Science of Concurrent Programs. Cambridge        *)
+(* > University Press.                                                        *)
+(* > https://doi.org/10.1017/9781009719841                                    *)
+(*                                                                            *)
+(* Other references:                                                          *)
+(* > Martin Abadi and Leslie Lamport. 1995. Conjoining Specifications. ACM    *)
+(* > Trans. Program. Lang. Syst. 17, 3 (May 1995), 507-535.                   *)
+(* > https://doi.org/10.1145/203095.201069                                    *)
+(* ========================================================================== *)
 
-Context {State : Type}.
-#[local] Notation prop := (property State).
+(* ========================================================================== *)
+(* Utility lemmas (local)                                                     *)
+(* ========================================================================== *)
+
+(* Ref: SCP Section 8.2.1.2 *)
+(* "F is true of the finite behavior \sigma(0) -> ... -> \sigma(k-1)" *)
+(* "For a safety property, true through state k means true if all states i with
+   i > k equal state k" *)
+(* Note: we define the tts operator by excluding the k'th state unlike SCP that
+   includes the k'th state *)
+Definition util_tts {State : Type} (P : property State) (beh : behavior State) (k : nat) : Prop :=
+    k = 0
+    \/ (exists beh' : behavior State,
+            P beh'
+            /\ (forall n : nat, n < k -> beh' n = beh n)).
+
+(* Ref: "Conjoining Specifications", section 3.4 *)
+(* The closure of F `C(F)` is defined "such that a behavior \sigma satisfies
+   C(F) iff every prefix of \sigma satisfies F". *)
+(* `\C(F)` *)
+Definition util_closure {State : Type} (F : property State) : property State :=
+    fun beh => forall n : nat, util_tts F beh n.
+
+(* Ref: "Conjoining Specifications", section 3.5 *)
+(* The "+ operator" is defined such that "a behavior \sigma satisfies E+v iff
+   either \sigma satisfies E, or there is some n such that (1) E holds for the
+   first n states of \sigma and (2) v never changes from the (n + 1)st state
+   on" *)
+(* `F_{+v}` *)
+Definition util_plus_operator {State V : Type} (F : property State) (v : State -> V) : property State :=
+    fun beh =>
+        F beh
+        \/ (exists k : nat,
+                (forall n : nat, k <= n -> v (beh n) = v (beh (S n)))
+                /\ util_tts F beh k).
 
 (* ========================================================================== *)
 (* Composition                                                                *)
 (* ========================================================================== *)
 
-(* Acyclic composition of `A` and `B` where `A` depends on the specification 
-   of `B` (and not the implementation of `B`). *)
-(* Note: not from references *)
-Lemma COM1 (A_i A_s B_i B_s : prop) :
-    valid (A_i \impl A_s)
-        -> valid ((A_s \land B_i) \impl B_s)
-            -> valid ((A_i \land B_i) \impl (A_s \land B_s)).
+Section rules.
+
+Context {State : Type}.
+#[local] Notation prop := (property State).
+
+(* Ref: SCP Theorem 8.7 (Decomposition Theorem) *)
+Theorem Decomposition {V : Type} (v : State -> V) (E Ml M : nat -> prop) :
+    (forall i : nat,
+            util_stuttering_closed (Ml i))  ->
+    (* If... *)
+    (* 1. *)
+    (forall i : nat,
+            valid ((\A j : (util_closure (M j)))
+                \impl (E i))) ->
+    (* 2. (a) *)
+    (forall i : nat,
+            valid (((util_plus_operator (util_closure (E i)) v) \land (util_closure (Ml i)))
+                \impl (util_closure (M i)))) ->
+    (* 2. (b) *)
+    (forall i : nat,
+            valid (((E i) \land ((Ml i) \land (\A j : ((LIFT0 (j < i)) \impl (M j)))))
+                \impl (M i))) ->
+    (* ...then *)
+    valid ((\A i : Ml i) \impl (\A i : M i)).
 Proof.
-    admit.
-Admitted.
+(* TODO *) Admitted.
+
+(* Not from refs *)
+(* Acyclic form of the `Decomposition` theorem with strenghtening of hypothesis 
+   (1.) by replacing `util_closure (M j)` with `M j` *)
+Theorem Decomposition0 (E Ml M : nat -> prop) :
+    (* If... *)
+    (* 1. *)
+    (forall i : nat,
+            valid ((\A j : ((LIFT0 (j < i)) \impl (M j)))
+                \impl (E i))) ->
+    (* 2. (b) *)
+    (forall i : nat,
+            valid (((E i) \land ((Ml i) \land (\A j : ((LIFT0 (j < i)) \impl (M j)))))
+                \impl (M i))) ->
+    (* ...then *)
+    valid ((\A i : Ml i) \impl (\A i : M i)).
+Proof.
+(* TODO *)  Admitted.
+
+(* Acyclic composition of `M0` and `M1` where `M1` depends on the specification 
+   of `M0` (and not the implementation `Ml0` of `M0`). *)
+(* Not from refs *)
+#[local] Example ex_01 (Ml0 M0 Ml1 M1 : prop) :
+    valid (Ml0  \impl  M0)  ->
+        valid ((M0 \land Ml1)  \impl  M1)  ->
+            valid ((Ml0 \land Ml1)  \impl  (M0 \land M1)).
+Proof.
+(* TODO *)  Admitted.
 
 End rules.
